---
layout:     series
title:      "Lines"
date:       2023-09-06
categories: blog moments-of-inertia
permalink:  ":categories/:title/"
part:       5
series:     moments-of-inertia
tags:       moments-of-inertia
excerpt_separator: <!--more-->
---

This is going to be a useful building block for future posts.

## Parameterizing the Curve

Suppose a line has its endpoints at $(x_1, y_1, z_1)$ and $(x_2, y_2, z_2)$.

$$
\b{r}(t) = ((x_2 - x_1) t + x_1) \; \u{x} + ((y_2 - y_1) t + y_1) \; \u{y} + ((z_2 - z_1) t + z_1) \; \u{z} 
$$

$$
d \b{\ell} = \frac{\partial \b{r}}{\partial t} dt = \left ( (x_2 - x_1) \; \u{x} + (y_2 - y_1) \; \u{y} + (z_2 - z_1) \; \u{z} \right ) \; dt
$$

$$
d\ell = \abs{d \b{\ell} } = \sqrt{(x_2 - x_1)^2 + (y_2 - y_1)^2 + (z_2 - z_1)^2} \; dt = L \; dt
$$

## Mass

$$
\begin{align}
    M &= \int dm \\[10pt]
    &= \lambda \int d\ell \\[10pt]
    &= \lambda \int_{0}^{1} L \; dt \\[10pt]
    &= \lambda L
\end{align}
$$

<br>

## General Line

We are going to calculate the inertia matrix. We will assume the axis of rotation is the $z$-axis. The other axes can be computed symmetrically.

$$
\begin{align}
    I_{zz} &= \int r_{axis}^2 dm \\[10pt]
    &= \lambda \int r_{axis}^2 d\ell \\[10pt]
    &= \lambda \int_{0}^{1} \left [ ((x_2 - x_1) t + x_1)^2 + ((y_2 - y_1) t + y_1)^2 \right ] \; L \; dt \\[10pt]
    &= \lambda \left [ \frac{x_2^3 - x_1^2}{3(x_2 - x_1)} + \frac{y_2^3 - y_1^2}{3(y_2 - y_1)} \right ] \; L \\[10pt]
    &= \tfrac{1}{3} M \left [ \frac{x_2^3 - x_1^2}{x_2 - x_1} + \frac{y_2^3 - y_1^2}{y_2 - y_1} \right ] \\[10pt]
    &= \tfrac{1}{3} M \left [ (x_1 + x_2)^2 + (y_1 + y_2)^2 + x_1x_2 + y_1y_2 \right ]
\end{align}
$$

Now we do the product of inertia.

$$
\begin{align}
    I_{xy} &= \int xy \; dm \\[10pt]
    &= \lambda \int xy \; d\ell \\[10pt]
    &= \lambda \int_{0}^{1} \left [ ((x_2 - x_1) t + x_1) \cdot ((y_2 - y_1) t + y_1) \right ] \; L \; dt \\[10pt]
    &= \lambda \left [ \tfrac{1}{3} (x_2 - x_1) (y_2 - y_1) + \tfrac{1}{2} x_1 (y_2 - y_1) + \tfrac{1}{2} (x_2 - x_1) y_1 + x_1 y_1 \right ] \; L \\[10pt]
    &= \tfrac{1}{6} \lambda \left [ (x_2 + x_1) (y_2 + y_1) + x_1y_1 + x_2y_2 \right ] \; L \\[10pt]
    &= \tfrac{1}{6} M \left [ (x_2 + x_1) (y_2 + y_1) + x_1y_1 + x_2y_2 \right ]
\end{align}
$$

Again, we can get $I_{yz}$ and $I_{zx}$ symmetrically. This gives the complete inertia tensor

<!-- 
$$
I = \begin{bmatrix}
    \tfrac{1}{3} M \left [ (y_1 + y_2)^2 + (z_1 + z_2)^2 + y_1y_2 + z_1z_2 \right ] & 0 & 0 \\
    0 & \tfrac{1}{3} M \left [ (z_1 + z_2)^2 + (x_1 + x_2)^2 + z_1z_2 + x_1x_2 \right ] & - \sin \gamma \\
    0 & \sin \gamma & \tfrac{1}{3} M \left [ (x_1 + x_2)^2 + (y_1 + y_2)^2 + x_1x_2 + y_1y_2 \right ]
\end{bmatrix}
$$ 
-->

<br>

## Special Cases

The above formulae look pretty nasty, but that's because they are very general. We can now take special cases in order to useful results

<br>

### Line about Perpendicular Axis at a Distance

Here, we use $I_{zz}$ and without loss of generality can assume the line is parallel to the $x$-axis. Therefore, $y_1 = y_2 = d$, $x_1 = -L/2$, $x_2 = L/2$.

$$
I = \tfrac{1}{3} \left [ ((-L/2) + (L/2))^2 + (d + d)^2 + (-L/2)(L/2) + (d)(d) \right ] = \tfrac{1}{12} M L^2 + M d^2
$$

This formula is suspiciously clean. We will see a generalized result later.

<br>

### Line about Perpendicular Axis at its Center

Here, we use $I_{zz}$ and without loss of generality can assume the line lies on the $x$-axis. Therefore, $y_1 = y_2 = 0$, $x_1 = -L/2$, $x_2 = L/2$.

$$
I = \tfrac{1}{3} \left [ ((-L/2) + (L/2))^2 + (0 + 0)^2 + (-L/2)(L/2) + (0)(0) \right ] = \tfrac{1}{12} M L^2
$$

<br>

### Line about Perpendicular Axis at its End

Here, we use $I_{zz}$ and without loss of generality can assume the line lies on the $x$-axis. Therefore, $y_1 = y_2 = 0$, $x_1 = 0$, $x_2 = L$.

$$
I = \tfrac{1}{3} \left [ (0 + L)^2 + (0 + 0)^2 + (0)(L) + (0)(0) \right ] = \tfrac{1}{3} M L^2
$$

